zoo_saturn/mpmc_bqueue: ocaml2zoo-ify.

lib/zoo_saturn/mpmc_bqueue.ml
@@ -1,0 +1,113 @@
+(* Based on:
+   https://github.com/ocaml-multicore/saturn/blob/306bea620cc0cfcc33639c45a56da59add9bdd92/src/bounded_queue/bounded_queue.body.ml
+*)
+
+type ('a, _) node =
+  | Null :
+    ('a, [> `Null]) node
+  | Node :
+    { mutable next: ('a, [`Null | `Node]) node [@atomic];
+      mutable data: 'a;
+      mutable index: int;
+      mutable estimated_capacity: int;
+    } ->
+    ('a, [> `Node]) node
+
+type 'a t =
+  { capacity: int;
+    mutable front: ('a, [`Node]) node [@atomic];
+    mutable back: ('a, [`Node]) node [@atomic];
+  }
+
+let create cap =
+  let front =
+    Node {
+      next= Obj.magic ();
+      data= Obj.magic ();
+      index= 0;
+      estimated_capacity= cap;
+    }
+  in
+  { capacity= cap; front; back= front }
+
+let capacity t =
+  t.capacity
+
+let rec size t =
+  let (Node front_r as front) = t.front in
+  let proph = Zoo.proph in
+  let (Node back_r as back) = t.back in
+  match back_r.next with
+  | Node _ as node ->
+      Atomic.Loc.compare_and_set [%atomic.loc t.back] back node |> ignore ;
+      size t
+  | Null ->
+      if Zoo.resolve t.front proph () != front then
+        size t
+      else
+        back_r.index - front_r.index
+
+let is_empty t =
+  let Node front_r = t.front in
+  front_r.next == Null
+
+let rec fix_back t back new_back =
+  let Node new_back_r = new_back in
+  if new_back_r.next == Null
+  && not @@ Atomic.Loc.compare_and_set [%atomic.loc t.back] back new_back
+  then (
+    Domain.yield () ;
+    fix_back t t.back new_back
+  )
+let rec push t back (new_back : (_, [`Node]) node) cap =
+  let Node back_r = back in
+  let (Node new_back_r as new_back) = new_back in
+  if cap = 0 then (
+    let Node front_r = t.front in
+    let cap = t.capacity - (back_r.index - front_r.index) in
+    if cap <= 0 then (
+      false
+    ) else (
+      back_r.estimated_capacity <- cap ;
+      push t back new_back cap
+    )
+  ) else (
+    new_back_r.index <- back_r.index + 1 ;
+    new_back_r.estimated_capacity <- cap - 1 ;
+    if Atomic.Loc.compare_and_set [%atomic.loc back_r.next] Null new_back then (
+      fix_back t back new_back ;
+      true
+    ) else (
+      match back_r.next with
+      | Null ->
+          assert false
+      | Node back_r as back ->
+          push t back new_back back_r.estimated_capacity
+    )
+  )
+let push t v =
+  let new_back =
+    Node {
+      next= Null;
+      data= v;
+      index= 0;
+      estimated_capacity= 0;
+    }
+  in
+  let Node back_r as back = t.back in
+  push t back new_back back_r.estimated_capacity
+
+let rec pop t =
+  let Node front_r as front = t.front in
+  match front_r.next with
+  | Null ->
+      None
+  | Node new_front_r as new_front ->
+      if Atomic.Loc.compare_and_set [%atomic.loc t.front] front new_front then (
+        let v = new_front_r.data in
+        new_front_r.data <- Obj.magic () ;
+        Some v
+      ) else (
+        Domain.yield () ;
+        pop t
+      )
