lib/zoo_saturn/mpmc_bqueue.mli
@@ -1,0 +1,19 @@
+type 'a t
+
+val create :
+  int -> 'a t
+
+val capacity :
+  'a t -> int
+
+val size :
+  'a t -> int
+
+val is_empty :
+  'a t -> bool
+
+val push :
+  'a t -> 'a -> bool
+
+val pop :
+  'a t -> 'a option
