theories/zoo_saturn/mpmc_bqueue.v
@@ -1,7 +1,3 @@
-(* Based on:
-   https://github.com/ocaml-multicore/saturn/blob/306bea620cc0cfcc33639c45a56da59add9bdd92/src/bounded_queue/bounded_queue.body.ml
-*)
-
 From zoo Require Import
   prelude.
 From zoo.language Require Import
@@ -9,116 +5,17 @@ From zoo.language Require Import
 From zoo.diaframe Require Import
   diaframe.
 From zoo_std Require Import
-  option
-  domain.
+  option.
 From zoo_saturn Require Export
-  base.
+  base
+  mpmc_bqueue__code.
+From zoo_saturn Require Import
+  mpmc_bqueue__types.
 From zoo Require Import
   options.
 
 Implicit Types v t : val.
 Implicit Types vs : list val.
-
-#[local] Notation "'node_next'" := (
-  in_type "node" 0
-)(in custom zoo_field
-).
-#[local] Notation "'node_data'" := (
-  in_type "node" 1
-)(in custom zoo_field
-).
-#[local] Notation "'node_capacity'" := (
-  in_type "node" 2
-)(in custom zoo_field
-).
-#[local] Notation "'node_count'" := (
-  in_type "node" 3
-)(in custom zoo_field
-).
-
-#[local] Notation "'capacity'" := (
-  in_type "t" 0
-)(in custom zoo_field
-).
-#[local] Notation "'front'" := (
-  in_type "t" 1
-)(in custom zoo_field
-).
-#[local] Notation "'back'" := (
-  in_type "t" 2
-)(in custom zoo_field
-).
-
-#[local] Definition node_create : val :=
-  fun: "v1" "v2" "v3" "v4" =>
-    { "v1", "v2", "v3", "v4" }.
-
-Definition mpmc_bqueue_create : val :=
-  fun: "cap" =>
-    let: "front" := node_create () () "cap" #0 in
-    { "cap", "front", "front" }.
-
-Definition mpmc_bqueue_capacity : val :=
-  fun: "t" =>
-    "t".{capacity}.
-
-Definition mpmc_bqueue_is_empty : val :=
-  fun: "t" =>
-    "t".{front}.{node_next} == ().
-
-#[local] Definition mpmc_bqueue_fix_back : val :=
-  rec: "mpmc_bqueue_fix_back" "t" "back" "new_back" =>
-    if: "new_back".{node_next} == () and ~ CAS "t".[back] "back" "new_back" then
-      "mpmc_bqueue_fix_back" "t" "t".{back} "new_back".
-#[local] Definition mpmc_bqueue_push_aux : val :=
-  rec: "mpmc_bqueue_push_aux" "t" "back" "new_back" "cap" =>
-    if: "cap" == #0 then (
-      let: "cap" := "t".{capacity} - ("back".{node_count} - "t".{front}.{node_count}) in
-      if: "cap" ≤ #0 then (
-        #false
-      ) else (
-        "back" <-{node_capacity} "cap" ;;
-        "mpmc_bqueue_push_aux" "t" "back" "new_back" "cap"
-      )
-    ) else (
-      "new_back" <-{node_capacity} "cap" - #1 ;;
-      "new_back" <-{node_count} "back".{node_count} + #1 ;;
-      if: CAS "back".[node_next] () "new_back" then (
-        mpmc_bqueue_fix_back "t" "back" "new_back" ;;
-        #true
-      ) else (
-        let: "back" := "back".{node_next} in
-        "mpmc_bqueue_push_aux" "t" "back" "new_back" "back".{node_capacity}
-      )
-    ).
-Definition mpmc_bqueue_push : val :=
-  fun: "t" "v" =>
-    let: "new_back" := node_create () "v" #0 #0 in
-    let: "back" := "t".{back} in
-    mpmc_bqueue_push_aux "t" "back" "new_back" "back".{node_capacity}.
-
-#[local] Definition mpmc_queue_do_push : val :=
-  rec: "mpmc_queue_do_push" "node" "new_back" =>
-    let: "node'" := "node".{node_next} in
-    if: "node'" != () or ~ CAS "node".[node_next] () "new_back" then
-      "mpmc_queue_do_push" "node'" "new_back".
-
-Definition mpmc_bqueue_pop : val :=
-  rec: "mpmc_bqueue_pop" "t" =>
-    let: "old_front" := "t".{front} in
-    let: "front" := "old_front".{node_next} in
-    if: "front" == () then (
-      §None
-    ) else (
-      if: CAS "t".[front] "old_front" "front" then (
-        let: "v" := "front".{node_data} in
-        "front" <-{node_data} () ;;
-        ‘Some{ "v" }
-      ) else (
-        domain_yield () ;;
-        "mpmc_bqueue_pop" "t"
-      )
-    ).
 
 Class MpmcBqueueG Σ `{zoo_G : !ZooG Σ} := {
 }.
@@ -160,6 +57,33 @@ Section mpmc_bqueue_G.
       mpmc_bqueue_inv t ι ₊cap ∗
       mpmc_bqueue_model t []
     }}}.
+  Proof.
+  Admitted.
+
+  Lemma mpmc_bqueue_capacity_spec t ι cap :
+    {{{
+      mpmc_bqueue_inv t ι cap
+    }}}
+      mpmc_bqueue_capacity t
+    {{{
+      RET #cap;
+      True
+    }}}.
+  Proof.
+  Admitted.
+
+  Lemma mpmc_bqueue_size_spec t ι cap :
+    <<<
+      mpmc_bqueue_inv t ι cap
+    | ∀∀ vs,
+      mpmc_bqueue_model t vs
+    >>>
+      mpmc_bqueue_size t
+    <<<
+      mpmc_bqueue_model t vs
+    | RET #(length vs);
+      True
+    >>>.
   Proof.
   Admitted.
 
@@ -211,6 +135,10 @@ End mpmc_bqueue_G.
 
 #[global] Opaque mpmc_bqueue_create.
 #[global] Opaque mpmc_bqueue_capacity.
+#[global] Opaque mpmc_bqueue_size.
 #[global] Opaque mpmc_bqueue_is_empty.
 #[global] Opaque mpmc_bqueue_push.
 #[global] Opaque mpmc_bqueue_pop.
+
+#[global] Opaque mpmc_bqueue_inv.
+#[global] Opaque mpmc_bqueue_model.
