theories/zoo_saturn/mpmc_bqueue__code.v
@@ -1,0 +1,142 @@
+From zoo Require Import
+  prelude.
+From zoo.language Require Import
+  typeclasses
+  notations.
+From zoo Require Import
+  structeq.
+From zoo_std Require Import
+  domain.
+From zoo_saturn Require Import
+  mpmc_bqueue__types.
+From zoo Require Import
+  options.
+
+Definition mpmc_bqueue_create : val :=
+  fun: "cap" =>
+    let: "front" := ‘Node{ (), (), #0, "cap" } in
+    { "cap", "front", "front" }.
+
+Definition mpmc_bqueue_capacity : val :=
+  fun: "t" =>
+    "t".{capacity}.
+
+Definition mpmc_bqueue_size : val :=
+  rec: "size" "t" =>
+    match: "t".{front} with
+    | Node <> <> <> <> as "front" =>
+        let: "front_r" := "front" in
+        let: "proph" := Proph in
+        match: "t".{back} with
+        | Node <> <> <> <> as "back" =>
+            let: "back_r" := "back" in
+            match: "back_r".{next} with
+            | Node <> <> <> <> as "node" =>
+                CAS "t".[back] "back" "node" ;;
+                "size" "t"
+            | Null =>
+                if: Resolve "t".{front} "proph" () != "front" then (
+                  "size" "t"
+                ) else (
+                  "back_r".{index} - "front_r".{index}
+                )
+            end
+        end
+    end.
+
+Definition mpmc_bqueue_is_empty : val :=
+  fun: "t" =>
+    match: "t".{front} with
+    | Node <> <> <> <> as "front_r" =>
+        "front_r".{next} == §Null
+    end.
+
+Definition mpmc_bqueue_fix_back : val :=
+  rec: "fix_back" "t" "back" "new_back" =>
+    match: "new_back" with
+    | Node <> <> <> <> as "new_back_r" =>
+        if:
+          "new_back_r".{next} == §Null and
+          ~ CAS "t".[back] "back" "new_back"
+        then (
+          domain_yield () ;;
+          "fix_back" "t" "t".{back} "new_back"
+        )
+    end.
+
+Definition mpmc_bqueue_push_0 : val :=
+  rec: "push" "t" "back" "new_back" "cap" =>
+    match: "back" with
+    | Node <> <> <> <> as "back_r" =>
+        match: "new_back" with
+        | Node <> <> <> <> as "new_back" =>
+            let: "new_back_r" := "new_back" in
+            if: "cap" = #0 then (
+              match: "t".{front} with
+              | Node <> <> <> <> as "front_r" =>
+                  let: "cap" :=
+                    "t".{capacity} - ("back_r".{index} - "front_r".{index})
+                  in
+                  if: "cap" ≤ #0 then (
+                    #false
+                  ) else (
+                    "back_r" <-{estimated_capacity} "cap" ;;
+                    "push" "t" "back" "new_back" "cap"
+                  )
+              end
+            ) else (
+              "new_back_r" <-{index} "back_r".{index} + #1 ;;
+              "new_back_r" <-{estimated_capacity} "cap" - #1 ;;
+              if: CAS "back_r".[next] §Null "new_back" then (
+                mpmc_bqueue_fix_back "t" "back" "new_back" ;;
+                #true
+              ) else (
+                match: "back_r".{next} with
+                | Null =>
+                    Fail
+                | Node <> <> <> <> as "back" =>
+                    let: "back_r" := "back" in
+                    "push"
+                      "t"
+                      "back"
+                      "new_back"
+                      "back_r".{estimated_capacity}
+                end
+              )
+            )
+        end
+    end.
+
+Definition mpmc_bqueue_push : val :=
+  fun: "t" "v" =>
+    let: "new_back" := ‘Node{ §Null, "v", #0, #0 } in
+    match: "t".{back} with
+    | Node <> <> <> <> as "back" =>
+        let: "back_r" := "back" in
+        mpmc_bqueue_push_0
+          "t"
+          "back"
+          "new_back"
+          "back_r".{estimated_capacity}
+    end.
+
+Definition mpmc_bqueue_pop : val :=
+  rec: "pop" "t" =>
+    match: "t".{front} with
+    | Node <> <> <> <> as "front" =>
+        let: "front_r" := "front" in
+        match: "front_r".{next} with
+        | Null =>
+            §None
+        | Node <> <> <> <> as "new_front" =>
+            let: "new_front_r" := "new_front" in
+            if: CAS "t".[front] "front" "new_front" then (
+              let: "v" := "new_front_r".{data} in
+              "new_front_r" <-{data} () ;;
+              ‘Some( "v" )
+            ) else (
+              domain_yield () ;;
+              "pop" "t"
+            )
+        end
+    end.
