theories/zoo_saturn/mpmc_bqueue__types.v
@@ -1,0 +1,50 @@
+From zoo Require Import
+  prelude.
+From zoo.language Require Import
+  typeclasses
+  notations.
+From zoo Require Import
+  structeq.
+From zoo_std Require Import
+  domain.
+From zoo Require Import
+  options.
+
+Notation "'Null'" := (
+  in_type "node" 0
+)(in custom zoo_tag
+).
+Notation "'Node'" := (
+  in_type "node" 1
+)(in custom zoo_tag
+).
+
+Notation "'next'" := (
+  in_type "node__Node" 0
+)(in custom zoo_field
+).
+Notation "'data'" := (
+  in_type "node__Node" 1
+)(in custom zoo_field
+).
+Notation "'index'" := (
+  in_type "node__Node" 2
+)(in custom zoo_field
+).
+Notation "'estimated_capacity'" := (
+  in_type "node__Node" 3
+)(in custom zoo_field
+).
+
+Notation "'capacity'" := (
+  in_type "t" 0
+)(in custom zoo_field
+).
+Notation "'front'" := (
+  in_type "t" 1
+)(in custom zoo_field
+).
+Notation "'back'" := (
+  in_type "t" 2
+)(in custom zoo_field
+).
